thy/Primitive_Matchers/Code_Interface.thy
@@ -23,34 +23,34 @@ section\<open>Code Interface\<close>
 text\<open>The parser returns the @{typ "'i::len common_primitive ruleset"} not as a map but as an association list.
       This function converts it\<close>
 (*TODO: this is IPv4 only currently*)
-definition map_of_string :: "(string \<times> 32 common_primitive rule list) list \<Rightarrow> string \<rightharpoonup> 32 common_primitive rule list" where
-  "map_of_string rs = map_of rs"
+definition map_of_string_ipv4 :: "(string \<times> 32 common_primitive rule list) list \<Rightarrow> string \<rightharpoonup> 32 common_primitive rule list" where
+  "map_of_string_ipv4 rs = map_of rs"
 
 
-definition unfold_ruleset_CHAIN_safe :: "string \<Rightarrow> action \<Rightarrow> 32 common_primitive ruleset \<Rightarrow> 32 common_primitive rule list option" where
+definition unfold_ruleset_CHAIN_safe :: "string \<Rightarrow> action \<Rightarrow> 'i::len common_primitive ruleset \<Rightarrow> 'i common_primitive rule list option" where
 "unfold_ruleset_CHAIN_safe = unfold_optimize_ruleset_CHAIN optimize_primitive_univ"
 
 lemma "(unfold_ruleset_CHAIN_safe chain a rs = Some rs') \<Longrightarrow> simple_ruleset rs'"
   by(simp add: Let_def unfold_ruleset_CHAIN_safe_def unfold_optimize_ruleset_CHAIN_def split: split_if_asm)
 
 (*TODO: This is just for legacy code compatibility. Use the new _safe function instead*)
-definition unfold_ruleset_CHAIN :: "string \<Rightarrow> action \<Rightarrow> 32 common_primitive ruleset \<Rightarrow> 32 common_primitive rule list" where
+definition unfold_ruleset_CHAIN :: "string \<Rightarrow> action \<Rightarrow> 'i::len common_primitive ruleset \<Rightarrow> 'i common_primitive rule list" where
   "unfold_ruleset_CHAIN chain default_action rs = the (unfold_ruleset_CHAIN_safe chain default_action rs)"
 
 
-definition unfold_ruleset_FORWARD :: "action \<Rightarrow> 32 common_primitive ruleset \<Rightarrow> 32 common_primitive rule list" where
+definition unfold_ruleset_FORWARD :: "action \<Rightarrow> 'i::len common_primitive ruleset \<Rightarrow> 'i::len common_primitive rule list" where
   "unfold_ruleset_FORWARD = unfold_ruleset_CHAIN ''FORWARD''"
 
-definition unfold_ruleset_INPUT :: "action \<Rightarrow> 32 common_primitive ruleset \<Rightarrow> 32 common_primitive rule list" where
+definition unfold_ruleset_INPUT :: "action \<Rightarrow> 'i::len common_primitive ruleset \<Rightarrow> 'i::len common_primitive rule list" where
   "unfold_ruleset_INPUT = unfold_ruleset_CHAIN ''INPUT''"
 
-definition unfold_ruleset_OUTPUT :: "action \<Rightarrow> 32 common_primitive ruleset \<Rightarrow> 32 common_primitive rule list" where
+definition unfold_ruleset_OUTPUT :: "action \<Rightarrow> 'i::len common_primitive ruleset \<Rightarrow> 'i::len common_primitive rule list" where
   "unfold_ruleset_OUTPUT \<equiv> unfold_ruleset_CHAIN ''OUTPUT''"
 
 
 lemma "let fw = [''FORWARD'' \<mapsto> []] in
   unfold_ruleset_FORWARD action.Drop fw
-  = [Rule MatchAny action.Drop]" by eval
+  = [Rule (MatchAny :: 32 common_primitive match_expr) action.Drop]" by eval
 
 
 (*
