thy/Examples/Parser_Test/Parser_Test.thy
@@ -141,7 +141,7 @@ value[code] "map (\<lambda>(c,rs). (c, map (common_primitive_rule_toString) rs))
 
 
 value[code] "let fw = (upper_closure (unfold_ruleset_FORWARD parser_test_firewall_FORWARD_default_policy
-                  (map_of_string (Semantics_Goto.rewrite_Goto parser_test_firewall))))
+                  (map_of_string_ipv4 (Semantics_Goto.rewrite_Goto parser_test_firewall))))
              in map common_primitive_rule_toString fw"
 
 text\<open>@{const abstract_for_simple_firewall} requires @{const normalized_nnf_match} primitives, 
@@ -149,18 +149,18 @@ text\<open>@{const abstract_for_simple_firewall} requires @{const normalized_nnf
       @{const has_unknowns}, therefore, @{const upper_closure} is called again.\<close>
 value[code] "(optimize_matches abstract_for_simple_firewall
                   (upper_closure (unfold_ruleset_FORWARD parser_test_firewall_FORWARD_default_policy
-                    (map_of_string (Semantics_Goto.rewrite_Goto parser_test_firewall)))))"
+                    (map_of_string_ipv4 (Semantics_Goto.rewrite_Goto parser_test_firewall)))))"
 
 value[code] "map simple_rule_toString (to_simple_firewall (upper_closure
                 (optimize_matches abstract_for_simple_firewall
                   (upper_closure (unfold_ruleset_FORWARD parser_test_firewall_FORWARD_default_policy
-                    (map_of_string (Semantics_Goto.rewrite_Goto parser_test_firewall)))))))" 
+                    (map_of_string_ipv4 (Semantics_Goto.rewrite_Goto parser_test_firewall)))))))" 
 
 
 value[code] "(optimize_matches abstract_for_simple_firewall
                   (upper_closure (packet_assume_new
                     (unfold_ruleset_FORWARD parser_test_firewall_FORWARD_default_policy
-                     (map_of_string (Semantics_Goto.rewrite_Goto parser_test_firewall))))))"
+                     (map_of_string_ipv4 (Semantics_Goto.rewrite_Goto parser_test_firewall))))))"
 
 
 hide_const parser_test_firewall
