thy/Examples/sns.ias.edu/SNS_IAS_Eduroam_Spoofing.thy
@@ -25,46 +25,46 @@ parse_iptables_save eduroam_fw="eduroam_iptables-save"
 thm eduroam_fw_def
 thm eduroam_fw_INPUT_default_policy_def
 
-value[code] "debug_ipassmt ipassignment_incoming (unfold_ruleset_INPUT eduroam_fw_INPUT_default_policy (map_of_string eduroam_fw))"
+value[code] "debug_ipassmt ipassignment_incoming (unfold_ruleset_INPUT eduroam_fw_INPUT_default_policy (map_of_string_ipv4 eduroam_fw))"
 
-value[code] "unfold_ruleset_INPUT eduroam_fw_INPUT_default_policy (map_of_string eduroam_fw)"
+value[code] "unfold_ruleset_INPUT eduroam_fw_INPUT_default_policy (map_of_string_ipv4 eduroam_fw)"
 
-value[code] "collect_ifaces (unfold_ruleset_INPUT eduroam_fw_INPUT_default_policy (map_of_string eduroam_fw))"
-
-
-lemma "ipassmt_sanity_defined (unfold_ruleset_INPUT eduroam_fw_INPUT_default_policy (map_of_string eduroam_fw)) (map_of_ipassmt ipassignment_incoming)" by eval
-lemma "ipassmt_sanity_defined (unfold_ruleset_OUTPUT eduroam_fw_OUTPUT_default_policy (map_of_string eduroam_fw)) (map_of_ipassmt ipassignment_outgoing)" by eval
+value[code] "collect_ifaces (unfold_ruleset_INPUT eduroam_fw_INPUT_default_policy (map_of_string_ipv4 eduroam_fw))"
 
 
-value[code] "debug_ipassmt ipassignment_incoming (unfold_ruleset_INPUT eduroam_fw_INPUT_default_policy (map_of_string eduroam_fw))"
-value[code] "debug_ipassmt ipassignment_outgoing (unfold_ruleset_OUTPUT eduroam_fw_OUTPUT_default_policy (map_of_string eduroam_fw))"
+lemma "ipassmt_sanity_defined (unfold_ruleset_INPUT eduroam_fw_INPUT_default_policy (map_of_string_ipv4 eduroam_fw)) (map_of_ipassmt ipassignment_incoming)" by eval
+lemma "ipassmt_sanity_defined (unfold_ruleset_OUTPUT eduroam_fw_OUTPUT_default_policy (map_of_string_ipv4 eduroam_fw)) (map_of_ipassmt ipassignment_outgoing)" by eval
+
+
+value[code] "debug_ipassmt ipassignment_incoming (unfold_ruleset_INPUT eduroam_fw_INPUT_default_policy (map_of_string_ipv4 eduroam_fw))"
+value[code] "debug_ipassmt ipassignment_outgoing (unfold_ruleset_OUTPUT eduroam_fw_OUTPUT_default_policy (map_of_string_ipv4 eduroam_fw))"
 
 
 text\<open>The ruleset\<close>
-lemma "check_simple_fw_preconditions (upper_closure (packet_assume_new (unfold_ruleset_INPUT eduroam_fw_INPUT_default_policy (map_of_string eduroam_fw))))" by eval
-value[code] "map simple_rule_toString (to_simple_firewall (upper_closure (packet_assume_new (unfold_ruleset_INPUT eduroam_fw_INPUT_default_policy (map_of_string eduroam_fw)))))"
-lemma "simple_fw_valid (to_simple_firewall (upper_closure (packet_assume_new (unfold_ruleset_INPUT eduroam_fw_INPUT_default_policy (map_of_string eduroam_fw)))))" by eval
-lemma "simple_fw_valid (to_simple_firewall (lower_closure (packet_assume_new (unfold_ruleset_INPUT eduroam_fw_INPUT_default_policy (map_of_string eduroam_fw)))))" by eval
+lemma "check_simple_fw_preconditions (upper_closure (packet_assume_new (unfold_ruleset_INPUT eduroam_fw_INPUT_default_policy (map_of_string_ipv4 eduroam_fw))))" by eval
+value[code] "map simple_rule_toString (to_simple_firewall (upper_closure (packet_assume_new (unfold_ruleset_INPUT eduroam_fw_INPUT_default_policy (map_of_string_ipv4 eduroam_fw)))))"
+lemma "simple_fw_valid (to_simple_firewall (upper_closure (packet_assume_new (unfold_ruleset_INPUT eduroam_fw_INPUT_default_policy (map_of_string_ipv4 eduroam_fw)))))" by eval
+lemma "simple_fw_valid (to_simple_firewall (lower_closure (packet_assume_new (unfold_ruleset_INPUT eduroam_fw_INPUT_default_policy (map_of_string_ipv4 eduroam_fw)))))" by eval
 
 
 text\<open>We do not need to call things such as @{const transform_optimize_dnf_strict} because the
      firewall already is in @{const normalized_nnf_match} (required for @{const no_spoofing_iface})\<close>
-lemma "transform_optimize_dnf_strict (unfold_ruleset_INPUT eduroam_fw_INPUT_default_policy (map_of_string eduroam_fw)) =
-          unfold_ruleset_INPUT action.Drop (map_of_string eduroam_fw)" by eval
+lemma "transform_optimize_dnf_strict (unfold_ruleset_INPUT eduroam_fw_INPUT_default_policy (map_of_string_ipv4 eduroam_fw)) =
+          unfold_ruleset_INPUT action.Drop (map_of_string_ipv4 eduroam_fw)" by eval
 
 text\<open>The ruleset prevents spoofed incoming packets\<close>
 lemma "no_spoofing_iface (Iface ''wlan0'')
-        (map_of_ipassmt ipassignment_incoming) (unfold_ruleset_INPUT eduroam_fw_INPUT_default_policy (map_of_string eduroam_fw))" by eval
+        (map_of_ipassmt ipassignment_incoming) (unfold_ruleset_INPUT eduroam_fw_INPUT_default_policy (map_of_string_ipv4 eduroam_fw))" by eval
 
 
 text\<open>Ruleset does not prevent that I'm spoofing (which is not necessary anyways since I need root right to spoof, which 
       would also enable me to deactivate the firewall). This is only a one-user laptop!\<close>
 
-lemma "transform_optimize_dnf_strict (unfold_ruleset_OUTPUT eduroam_fw_INPUT_default_policy (map_of_string eduroam_fw)) =
-        unfold_ruleset_OUTPUT eduroam_fw_INPUT_default_policy (map_of_string eduroam_fw)" by eval
+lemma "transform_optimize_dnf_strict (unfold_ruleset_OUTPUT eduroam_fw_INPUT_default_policy (map_of_string_ipv4 eduroam_fw)) =
+        unfold_ruleset_OUTPUT eduroam_fw_INPUT_default_policy (map_of_string_ipv4 eduroam_fw)" by eval
 
 lemma "\<not> no_spoofing_iface (Iface ''wlan0'')
-        (map_of_ipassmt ipassignment_outgoing) (unfold_ruleset_OUTPUT eduroam_fw_INPUT_default_policy (map_of_string eduroam_fw))" by eval
+        (map_of_ipassmt ipassignment_outgoing) (unfold_ruleset_OUTPUT eduroam_fw_INPUT_default_policy (map_of_string_ipv4 eduroam_fw))" by eval
 
 
 end
